KAT/KAT_rKAT_rVCs_ndfun.thy
@@ -418,6 +418,7 @@ lemma
 
 (****** SDF: Adapted this far *****)
 
+(*
 context local_flow
 begin
 
@@ -499,11 +500,13 @@ proof(subst ndfun_kat_H, simp add: g_orbital_eq p2ndf_def g_ode_def, clarsimp)
   thus "Q (X t)"
     using \<open>P s\<close> wp_Q by (subst (asm) ndfun_kat_H) (auto simp: g_ode_def)
 qed
+*)
 
 abbreviation g_global_ode ::"(('a::banach)\<Rightarrow>'a) \<Rightarrow> 'a pred \<Rightarrow> 'a nd_fun" ("(1x\<acute>=_ & _)") 
   where "(x\<acute>= f & G) \<equiv> (x\<acute>= f & G on UNIV UNIV @ 0)"
 
 abbreviation g_global_ode_inv :: "(('a::banach)\<Rightarrow>'a) \<Rightarrow> 'a pred \<Rightarrow> 'a pred \<Rightarrow> 'a nd_fun" 
   ("(1x\<acute>=_ & _ DINV _)") where "(x\<acute>= f & G DINV I) \<equiv> (x\<acute>= f & G on UNIV UNIV @ 0 DINV I)"
+
 
 end
